crates/move-prover-boogie-backend/src/boogie_backend/prelude/native.bpl
@@ -983,6 +983,17 @@ axiom (forall {{QP}}:: {$MapQuantifierHelper_{{FN}}({{QA}})}
 );
 {%- endif %}
 
+{%- if instance.qht == "range_map" %}
+function $RangeMapQuantifierHelper_{{FN}}({{QP}}): Vec ({{RT}});
+axiom (forall {{QP}}:: {$RangeMapQuantifierHelper_{{FN}}({{QA}})}
+(
+    var res := $RangeMapQuantifierHelper_{{FN}}({{QA}});
+        LenVec(res) == end - start &&
+        (forall i: int :: start <= i && i < end ==> ReadVec(res, i - start) == {{FN}}({{EAB}}i{{EAA}}))
+    )
+);
+{%- endif %}
+
 {% endmacro quantifier_helpers_module %}
 
 {% macro dynamic_field_key_module(impl, instance) %}
